uhoh, we're going to have to handle tactic_state ourselves

src/tactic/back.lean
@@ -3,7 +3,6 @@
 -- Authors: Scott Morrison, Keeley Hoek
 
 import tactic.basic
-import data.list.basic
 
 namespace tactic
 
@@ -58,9 +57,18 @@ meta structure back_state :=
 (committed   : list apply_state := {}) -- Stores goals which we must complete.
 (in_progress : list apply_state)       -- Stores goals which we're still working on.
 
+meta instance : has_to_string back_state :=
+{ to_string := λ s, to_string format!"back_state: {s.stashed.length}/{s.completed.length}/{s.committed.length}/{s.in_progress.length}" }
+
+meta instance has_to_tactic_format_back_state : has_to_tactic_format back_state :=
+{ to_tactic_format := λ s,
+    do return $ to_string s }
+
 -- TODO Think hard about what goes here; possibly allow customisation.
 meta def back_state.complexity (s : back_state) : ℕ × ℕ × ℕ :=
-(s.committed.length, s.in_progress.length, s.steps)
+-- (s.committed.length, s.in_progress.length, s.steps)
+-- It seems essential to put in_progress first, or we don't work hard enough.
+(s.in_progress.length, s.committed.length, s.steps) -- this is probably better??
 
 meta def back_state.done (s : back_state) : bool :=
 s.committed.empty ∧ s.in_progress.empty
@@ -85,12 +93,12 @@ meta def sort_by_arrows (L : list back_lemma) : tactic (list back_lemma) :=
 do M ← L.mmap (λ e, do c ← count_arrows <$> infer_type e.lem, return (c, e)),
    return ((list.qsort (λ (p q : ℕ × back_lemma), p.1 ≤ q.1) M).map (λ p, p.2))
 
-meta def back_state.init (progress finishing : list expr) (limit : option ℕ): tactic back_state :=
-do g :: _ ← get_goals,
+meta def back_state.init (goal : expr) (progress finishing : list expr) (limit : option ℕ): tactic back_state :=
+do
    -- We sort the lemmas, preferring lemmas which, when applied, will produce fewer new goals.
    lemmas ← sort_by_arrows $ (finishing.enum.map (λ e, ⟨e.2, tt, e.1⟩)) ++
                              (progress.enum.map  (λ e, ⟨e.2, ff, e.1 + finishing.length⟩)),
-   gmvar ← mk_goal_mvar g,
+   gmvar ← mk_goal_mvar goal,
    return
    { limit       := limit,
      lemmas      := lemmas,
@@ -116,7 +124,7 @@ do let s := (list.repeat ' ' n).as_string,
 * increment the `step` counter,
 * and remove applied iffs.
 -/
-meta def back_state.clean (s : back_state) (last_lemma : back_lemma) : tactic back_state :=
+meta def back_state.clean (s : back_state) (g : goal_mvar) (last_lemma : back_lemma) : tactic back_state :=
 do (stashed, completed_1) ← partition_mvars s.stashed,
    (committed, completed_2)   ← partition_apply_state_mvars s.committed,
    (in_progress, completed_3) ← partition_apply_state_mvars s.in_progress,
@@ -127,20 +135,22 @@ do (stashed, completed_1) ← partition_mvars s.stashed,
    return
    { steps       := s.steps + 1,
      stashed     := stashed,
-     completed   := completed,
+     completed   := g :: completed,
      committed   := committed,
      in_progress := in_progress,
      lemmas      := lemmas,
      .. s}
 
-meta def back_state.apply_lemma (s : back_state) (e : back_lemma) (committed : bool) : tactic back_state :=
+meta def back_state.apply_lemma (s : back_state) (g : goal_mvar) (e : back_lemma) (committed : bool) : tactic back_state :=
 do trace $ "attempting to apply " ++ to_string e.lem,
    get_goals >>= λ gs, gs.mmap infer_type >>= pad_trace s.steps,
   apply_thorough e.lem,
   trace "!",
+   get_goals >>= λ gs, gs.mmap infer_type >>= pad_trace s.steps,
   --  goal_types ← get_goals >>= λ gs, gs.mmap infer_type,
   --  pad_trace s.steps e,
-   s' ← s.clean e,
+   s' ← s.clean g e,
+   trace "cleaned",
    (done >> return s') <|> do
    gs ← get_goals,
    as ← gs.mmap $ λ g, (do gmvar ← mk_goal_mvar g, return (⟨gmvar, s.lemmas⟩ : apply_state)),
@@ -153,7 +163,7 @@ meta def back_state.apply (s : back_state) (committed : bool) : apply_state → 
 | as :=
   match as.lemmas with
   | [] := fail "No lemmas applied to the current goal."
-  | (h :: t) := do r ← try_core $ s.apply_lemma h committed,
+  | (h :: t) := do r ← try_core $ s.apply_lemma as.goal h committed,
                    match r with
                    | none := back_state.apply ⟨as.goal, t⟩
                    | (some bs) := do ng ← as.goal.new_mvars,
@@ -161,25 +171,30 @@ meta def back_state.apply (s : back_state) (committed : bool) : apply_state → 
                    end
   end
 
-meta def back_state.children (s : back_state) : tactic (list back_state) :=
-do
-match s.committed with
-| [] :=
-  -- Let's see if we can do anything with `in_progress` goals
-  match s.in_progress with
-  | [] := undefined
-  | (p :: ps) :=
+meta def back_state.apply_in_progress (s : back_state) : tactic (list back_state) :=
+match s.in_progress with
+| [] := undefined
+| (p :: ps) :=
   do set_goals [p.goal.synthetic],
-     s.apply ff p <|>
-     return [{ in_progress := ps, stashed := p.goal :: s.stashed, .. s }]
-  end
+     let s' := { in_progress := ps, ..s },
+     s'.apply ff p <|>
+     return (if s'.steps > 0 then [{ stashed := p.goal :: s'.stashed, .. s' }] else [])
+end
+
+meta def back_state.apply_committed (s : back_state) : tactic (list back_state) :=
+match s.committed with
+| [] := undefined
 | (c :: cs) :=
   -- We must discharge `c`.
   do set_goals [c.goal.synthetic],
-     s.apply tt c <|> return []
+     let s' := { committed := cs, ..s },
+     s'.apply tt c <|> return []
 end
 
-def lexicographic_preorder {α β : Type*} [preorder α] [decidable_eq α] [preorder β] : preorder (α × β) :=
+meta def back_state.children (s : back_state) : tactic (list back_state) :=
+if s.committed.empty then s.apply_in_progress else s.apply_committed
+
+def lexicographic_preorder {α β : Type*} [preorder α] [preorder β] : preorder (α × β) :=
 { le := λ a b, a.1 < b.1 ∨ (a.1 = b.1 ∧ a.2 ≤ b.2),
   le_refl := λ a, or.inr ⟨rfl, le_refl _⟩,
   le_trans := λ a b c h₁ h₂,
@@ -192,9 +207,12 @@ def lexicographic_preorder {α β : Type*} [preorder α] [decidable_eq α] [preo
       { rwa ←h₂.left } },
     { cases h₂,
       { left, rwa h₁.left },
-      { exact or.inr ⟨eq.trans h₁.1 h₂.1, le_trans h₁.2 h₂.2⟩ }
+      { right, exact ⟨eq.trans h₁.1 h₂.1, le_trans h₁.2 h₂.2⟩ }
     } end }
 local attribute [instance] lexicographic_preorder
+
+-- Just a check that we're actually using lexicographic ordering here.
+example : (5,10) < (10,3) := by exact dec_trivial
 
 private meta def insert_new_state : back_state → list back_state → list back_state
 /- depth first search: -/
@@ -218,35 +236,19 @@ private meta def run_one_step : list back_state → tactic (back_state ⊕ (list
     return $ sum.inl h
   else
     do c ← h.children,
+       trace "children:",
+       trace c,
        return $ sum.inr $ insert_new_states c t
 
 private meta def run : list back_state → tactic back_state
 | states :=
-  do r ← run_one_step states,
+  do trace "run:",
+     trace states,
+     r ← run_one_step states,
      match r with
      | (sum.inl success) := return success
      | (sum.inr states) := run states
      end
-
--- meta def back_state.run : back_state → tactic back_state
--- | s :=
---   do
---   guard (s.steps ≤ s.limit.get_or_else 20),
---   match s.committed with
---   | [] :=
---     -- Let's see if we can do anything with `in_progress` goals
---     match s.in_progress with
---     | [] := return s -- Great, all done!
---     | (p :: ps) :=
---     do set_goals [p],
---       (s.lemmas.enum.any_of $ λ e, { in_progress := ps, .. s }.apply e.1 e.2.1 e.2.2 >>= back_state.run)
---       <|> { in_progress := ps, stashed := p :: s.stashed, .. s }.run
---     end
---   | (c :: cs) :=
---     -- We must discharge `c`.
---     do set_goals [c],
---       s.lemmas.enum.any_of $ λ e, { committed := cs, .. s }.apply e.1 e.2.1 tt >>= back_state.run
---   end
 
 /-- Takes two sets of lemmas, 'progress' lemmas and 'finishing' lemmas.
 
@@ -256,11 +258,16 @@ private meta def run : list back_state → tactic back_state
     `back` succeeds if at least one progress lemma was applied, or all goals are discharged.
     -/
 meta def back (progress finishing : list expr) (limit : option ℕ) : tactic unit :=
-do i ← back_state.init progress finishing limit,
+do g :: gs ← get_goals,
+   i ← back_state.init g progress finishing limit,
    f ← run [i],
+   set_goals [g],
+  --  f.completed.mmap (λ g, instantiate_mvars g.synthetic >>= unify g.original),
+  --  f.stashed.mmap   (λ g, instantiate_mvars g.synthetic >>= unify g.original),
    f.completed.mmap (λ g, unify g.original g.synthetic),
    f.stashed.mmap   (λ g, unify g.original g.synthetic),
-   set_goals (f.stashed.map(goal_mvar.original)),
+   g ← instantiate_mvars g,
+   set_goals (g.list_meta_vars ++ gs),
    guard (f.steps > 0) -- Make sure some progress was made.
 
 private meta def lookup_tagged_lemma (n : name) : tactic (bool × expr) :=
@@ -407,7 +414,7 @@ meta def back
   (hs : parse back_arg_list) (wth : parse with_back_ident_list) (limit : parse (optional small_nat)) : tactic string :=
 do g :: _ ← get_goals,
    (pr, fi) ← tactic.mk_assumption_set no_dflt hs wth,
-   r ← focus1 $ (do
+   r ← (do
      tactic.back pr fi limit,
      g ← instantiate_mvars g,
      r ← pp (replace_mvars g),
