test/back.lean
@@ -11,28 +11,27 @@ begin
 end
 
 example {P : Prop} (h : P) : P :=
-by back
+by back?
 
 example {P Q : Prop} (h₁ : P) (h₂ : Q) : P :=
-by back
+by back?
 
 example {P Q : Prop} (h₁ : P) (h₂ : Q) : Q :=
-by back
+by back?
 
 example {P Q : Prop} (h₁ : P) (h₂ : P → Q) : Q :=
-by back
+by back?
 
 example {P Q R : Prop} (h₁ : P) (h₂ : P → Q) (h₃ : R → Q) : Q :=
-by back
+by back?
 
 example {P Q R : Prop} (h₁ : R) (h₂ : P → Q) (h₃ : R → Q) : Q :=
-by back
+by back?
 
 -- Verify that `back` uses `congr_arg`.
 example (f : ℕ → ℕ) (x y : ℕ) (p : x = y) : f x = f y :=
 begin
   success_if_fail { back [-congr_arg] },
-  apply congr_fun,
   back,
 end
 
@@ -47,7 +46,7 @@ theorem infinitude_of_primes (N : ℕ) : ∃ p ≥ N, prime p :=
 begin
   let M := fact N + 1,
   let p := min_fac M,
-  have pp : prime p, { back [ne_of_gt], },
+  have pp : prime p, { back? [ne_of_gt], },
   -- Adding a `?`, i.e. as `back? [ne_of_gt]`, reports the expression back built:
   -- exact min_fac_prime (ne_of_gt (succ_lt_succ (fact_pos N)))
   use p,
@@ -72,7 +71,7 @@ theorem infinitude_of_primes' (N : ℕ) : ∃ p ≥ N, prime p :=
 begin
   let M := fact N + 1,
   let p := min_fac M,
-  have pp : prime p, { back },
+  have pp : prime p, { back, },
   use p,
   split,
   {
